examples/fac_master/tzwrap/minter/AssetsAdmin.v
@@ -1,6 +1,6 @@
 Require Import Tokens_Lib.
 Require Import Blockchain.
-Require Import FA2InterfaceOwn.
+Require Import FA2Interface_Wrap.
 Require Import ZArith.
 Require Import Storage.
 Require Import List.
