examples/fac_master/tzwrap/minter/Tokens_Lib.v
@@ -1,7 +1,7 @@
 Require Import Ethereum_Lib.
 Require Import Storage.
 Require Import Blockchain.
-Require Import FA2InterfaceOwn.
+Require Import FA2Interface_Wrap.
 From ConCert.Examples Require Import FA2Interface.
 From ConCert.Execution Require Import Containers.
 Require Import Types.
